virtual functions axioms from FM dev meeting
- generating virtual function tables from cpp2v
- defining a (usable?) abstraction on top of virtual functions

cpp2v-tests/test_init_list.cpp
@@ -1,0 +1,22 @@
+struct A {
+    A() {}
+    A(int) {}
+    virtual int foo() { return 0; }
+};
+struct B : public A {
+    B(int) {}
+    B() {}
+    //virtual int foo() { return 3; }
+};
+
+struct C : public B {
+    int y;
+    int x;
+    C():x(0),y(7) {}
+    virtual int foo() { return 1; }
+};
+
+int test(C* c) {
+    B* b = static_cast<B*>(c);
+    return b->foo() + b->A::foo();
+}
