cpp2v-tests/test_virtual.cpp
@@ -1,0 +1,12 @@
+struct A {
+    virtual int f() const = 0;
+};
+
+struct B : public A {
+    virtual int f() const { return 0; }
+};
+
+
+int call(const A* a) {
+    return a->f();
+}
