theories/IrisBridge.v
@@ -48,7 +48,7 @@ Module ChargeNotation.
   (* Notation "'|>' P" := (▷  P)%I (at level 71). *)
   Notation "|> P" := (▷  P)%I (at level 20, right associativity).
 
-  Infix "-|-"  := (≡)%I (at level 85, no associativity).
+  Notation "P -|- Q"  := (P%I ≡ Q%I) (at level 85, no associativity).
   Notation "'[|'  P  '|]'" := (only_provable P).
 
 End ChargeNotation.
