theories/lang/cpp/logic/dispatch.v
@@ -1,0 +1,71 @@
+(*
+ * Copyright (C) BedRock Systems Inc. 2020 Gregory Malecha
+ *
+ * SPDX-License-Identifier:AGPL-3.0-or-later
+ *)
+(**
+ * reflecting virtual function dispatch in the logic.
+ *)
+Require Import bedrock.lang.cpp.ast.
+Require Import bedrock.lang.cpp.semantics.
+From bedrock.lang.cpp.logic Require Import pred heap_pred path_pred.
+Require Import bedrock.lang.cpp.logic.wp.
+
+Section with_cpp.
+  Context `{Σ : cpp_logic}.
+
+  (* the [Offset] to cast a [base] to a [derived] *)
+  Fixpoint base_to_derived  `(d : class_derives σ derived base) : Offset :=
+    match d with
+    | Derives_here st _ => _id
+    | Derives_base base st _ _ _ _ d =>
+      _dot (base_to_derived d) (_derived σ base derived)
+    end.
+
+  (* the [Offset] to cast a [derived] to a [base] *)
+  Fixpoint derived_to_base `(d : class_derives σ derived base) : Offset :=
+    match d with
+    | Derives_here st _ => _id
+    | Derives_base base st _ _ _ _ d =>
+      _dot (_base σ derived base) (derived_to_base d)
+    end.
+
+  Definition get_impl `(r : class_derives σ mdc tcls) (f : obj_name)
+    : option (ptr * Offset) :=
+    let override := (dispatch σ r f).1 in
+    match override.(vimpl) with
+    | None => None
+    | Some s => match glob_addr σ s with
+               | None => None
+               | Some p => Some (p, base_to_derived override.(derivation))
+               end
+    end.
+
+  (** [resolve_virtual σ this cls f Q] returns [Q fa this'] if resolving [f] on
+   * [this] results in a function that is equivalent to calling the pointer [fa]
+   * passing [this'] as the "this" argument.
+   *)
+  Definition resolve_virtual {σ : genv}
+             (this : Loc) (cls : globname) (f : obj_name)
+             (Q : forall (faddr this_addr : ptr), mpred) : mpred :=
+    Exists σ' mdc (pf : class_derives σ' mdc cls),
+        (* ^ we quantify over another program environment because class
+             extension is open, the caller does not need to know the target
+             function.
+           - the [class_derives] fact *must* be in [σ'] because [mdc] might
+             not exist in [σ].
+         *)
+      (Exists q, _at this (_identity σ' cls (Some mdc) q) **
+                 [| class_compatible σ.(genv_tu) σ'.(genv_tu) cls |] ** ltrue) //\\
+              (* ^ the [class_compatible σ' mdc cls] ensures that the virtual
+                   tables the [cls] class are compatible between the (possibly
+                   different) translation units.
+               *)
+      match get_impl pf f with
+      | Some (fa, off) =>
+        Exists p, _offsetL off this &~ p ** Q fa p
+      | None => (* the function wasn't found or the implemenation was pure virtual *)
+        lfalse
+      end.
+
+End with_cpp.
