theories/lang/cpp/semantics.v
@@ -1,9 +1,12 @@
 (*
- * Copyright (C) BedRock Systems Inc. 2019 Gregory Malecha
+ * Copyright (C) BedRock Systems Inc. 2019-2020 Gregory Malecha
  *
  * SPDX-License-Identifier: LGPL-2.1 WITH BedRock Exception for use over network, see repository root for details.
  *)
 From bedrock.lang.cpp.semantics Require Export
      sub_module
      values
-     operator.
+     operator
+     intensional
+     subtyping
+     dispatch.
