theories/lang/cpp/semantics/dispatch.v
@@ -1,0 +1,50 @@
+(*
+ * Copyright (C) BedRock Systems Inc. 2020 Gregory Malecha
+ *
+ * SPDX-License-Identifier:AGPL-3.0-or-later
+ *)
+Require Import stdpp.decidable.
+Require Import bedrock.lang.cpp.ast.
+Require Import bedrock.lang.cpp.semantics.values.
+Require Import bedrock.lang.cpp.semantics.subtyping.
+
+Record vhandle {σ : genv} : Set :=
+  { vimpl      : option obj_name
+  ; voverrider : globname
+  ; vfrom      : globname
+  ; derivation : class_derives σ voverrider vfrom }.
+Arguments vhandle σ : clear implicits.
+
+Section dispatch.
+  Context (σ : genv).
+
+  Definition list_get {T} (t : obj_name) (l : list (obj_name * T)) : option T :=
+    match
+      List.find (fun '(t',_) =>
+                   if decide (t = t') then true else false) l
+    with
+    | None => None
+    | Some (_, k) => Some k
+    end.
+
+  Fixpoint dispatch `(d : class_derives σ mdc from) (final : obj_name)
+    : vhandle σ * obj_name :=
+    match d with
+    | Derives_here st _ =>
+      ({| vimpl := mjoin (list_get final st.(s_virtuals))
+        ; voverrider := mdc
+        ; vfrom := from
+        ; derivation := d |}, final)
+    | Derives_base base st _ _ _ _ d' =>
+      let '(result, cand) := dispatch d' final in
+      match list_get cand st.(s_overrides) with
+      | None => (result, cand)
+      | Some cand =>
+        ({| vimpl := mjoin (list_get final st.(s_virtuals))
+          ; voverrider := mdc
+          ; vfrom := from
+          ; derivation := d |}, cand)
+      end
+    end.
+
+End dispatch.
