theories/lang/cpp/semantics/subtyping.v
@@ -1,0 +1,44 @@
+(*
+ * Copyright (C) BedRock Systems Inc. 2020 Gregory Malecha
+ *
+ * SPDX-License-Identifier:AGPL-3.0-or-later
+ *)
+
+(*
+ * This file defines various class relationships that are used in C++,
+ * mostly around sub-typing and virtual dispatch.
+ *
+ * todo: this should build on Tahina's work
+ *   http://gallium.inria.fr/~tramanan/cpp/thesis/thesis.pdf
+ *)
+Require Import stdpp.fin_maps.
+Require Import bedrock.lang.cpp.ast.
+Require Import bedrock.lang.cpp.semantics.values.
+
+Section extends.
+  Context (σ : genv).
+
+  (** [class_derives mdc cls] is a/the proof that [mdc] is a derived class
+      of [cls] (equivalently, [cls] is a base class of [mdc])
+
+      note that this definition is in [Set] allowing us to compute over it.
+   *)
+  Inductive class_derives (derived : globname) : globname -> Set :=
+  | Derives_here {st}
+      {_ : σ.(genv_tu).(globals) !! derived = Some (Gstruct st)}
+    : class_derives derived derived
+
+  | Derives_base base {st li result}
+      {_ : σ.(genv_tu).(globals) !! derived = Some (Gstruct st)}
+      {_ : In (base, li) st.(s_bases)}
+      (_ : class_derives base result)
+    : class_derives derived result
+
+  (* this could be extended for virtuals *)
+  .
+
+End extends.
+
+Arguments Derives_here {_ _} _ _.
+Arguments Derives_base {_ _} _.
+Arguments class_derives σ derived base : rename.
